prove aes_data_put_wait

investigations/bedrock2/Aes/Aes.v
@@ -150,7 +150,6 @@ Section Impl.
       }
     ))).
 
-
   (**** aes.c
     bool aes_data_ready(void) {
       return (REG32(AES_STATUS(0)) & (0x1u << AES_STATUS_INPUT_READY));
@@ -191,5 +190,28 @@ Section Impl.
      (aes_globals ++ [], [out], bedrock_func_body:(
       io! status = READ (AES_STATUS) ;
       out = status & (1 << AES_STATUS_IDLE)
+    ))).
+
+  (**** aes.c
+    void aes_data_put_wait(const void *data) {
+      // Wait for AES unit to be ready for new input data.
+      while (!aes_data_ready()) {
+      }
+
+      // Provide the input data.
+      aes_data_put(data);
+    }
+   ***)
+  Definition aes_data_put_wait : func :=
+    let data := "data" in
+    let is_ready := "is_ready" in
+    ("b2_data_put_wait",
+     (aes_globals ++ [data], [], bedrock_func_body:(
+      is_ready = 0 ;
+      while (is_ready == 0) {
+        unpack! is_ready = aes_data_ready coq:(aes_globals)
+      };
+
+      aes_data_put coq:(aes_globals ++ [expr.var data])
     ))).
 End Impl.
